(WIP) trying to sort splitOWNRSroundPivot - about to refactor to try starting with onnsiders (ownrs inside pivot)

TRUMP.dfy
@@ -4,13 +4,13 @@ include "Ownership-Parallel.dfy"
 
 
 lemma fromTheManyOne(less : seq<nat>, more : seq<nat>)
-   requires |less| == |more|
-   requires forall x | 0 <= x < |less| :: less[x] <= more[x]
-    ensures sum(less) <= sum(more)
-    {}
+  requires |less| == |more|
+  requires forall x | 0 <= x < |less| :: less[x] <= more[x]
+  ensures sum(less) <= sum(more)
+{}
 
 function sum(s : seq<int>) : int
-  { if (|s| == 0) then 0 else s[0] + sum(s[1..]) }
+{ if (|s| == 0) then 0 else s[0] + sum(s[1..]) }
 
 
 
@@ -56,66 +56,59 @@ function sum(s : seq<int>) : int
 
 
 lemma smooveKlonerator(divot : Object, pivot : Object, rivet : Object, blivet : Object, m : Klon)
- //given that pivot is cloned to blivet
- //lets see if partitioning owners across the pivot works
-   requires divot.Ready()
-   requires pivot.Ready()
-   requires rivet.Ready()
-   requires blivet.Ready()
+  //given that pivot is cloned to blivet
+  //lets see if partitioning owners across the pivot works
+  requires divot.Ready()
+  requires pivot.Ready()
+  requires rivet.Ready()
+  requires blivet.Ready()
 
-   requires klonReady(m)
-   requires klonCalid(m)
+  requires klonReady(m)
+  requires klonCalid(m)
 
-   requires pivot  == m.o
-   requires blivet == m.c
+  requires pivot  == m.o
+  requires blivet == m.c
 
-   requires strictlyInside(divot, pivot)
-   requires m.objectInKlown(divot)
-   requires m.m[pivot] == blivet   //is this too much already?
-   requires m.m[divot] == rivet    //is this too much already already?
+  requires strictlyInside(divot, pivot)
+  requires m.objectInKlown(divot)
+  requires m.m[pivot] == blivet   //is this too much already?
+  requires m.m[divot] == rivet    //is this too much already already?
 
-    ensures klonLine(divot,rivet,m)
-    ensures strictlyInside(rivet, blivet)
+  ensures klonLine(divot,rivet,m)
+  ensures strictlyInside(rivet, blivet)
 
 {
-      assert klonCalid(m);
-      assert klonAllLines(m);
-      assert klonLine(divot,rivet,m);
-      assert strictlyInside(divot, pivot);
-      assert divot != pivot;
-      assert klonIdentity(divot,rivet,m);
-      assert divot.AMFO <= m.m.Keys;
-      assert forall o <- divot.AMFO :: klonLine(o,m.m[o],m);
-      assert mapThruKlon(divot.owner, m) == rivet.owner;
+  assert klonCalid(m);
+  assert klonAllLines(m);
+  assert klonLine(divot,rivet,m);
+  assert strictlyInside(divot, pivot);
+  assert divot != pivot;
+  assert klonIdentity(divot,rivet,m);
+  assert divot.AMFO <= m.m.Keys;
+  assert forall o <- divot.AMFO :: klonLine(o,m.m[o],m);
+  assert mapThruKlon(divot.owner, m) == rivet.owner;
 
- var divotInside,divotOutside,divotFringe := splitOwnersAroundPivot(divot, pivot);
- assert pivot in divotFringe;
- var divotFringeNoPivot := divotFringe - {pivot};
+  //       var divotInside,divotOutside,divotFringe := splitOwnersAroundPivot(divot, pivot);
+  //       assert pivot in divotFringe;
+  //       var divotFringeNoPivot := divotFringe - {pivot};
+  //
+  //       var rivetInside,rivetOutside,rivetFringe := splitOwnersAroundPivot(rivet, blivet);
+  //       assert blivet in rivetFringe;
+  //       var rivetFringeNoPivot := rivetFringe - {blivet};
+  //
+  //       assert forall o <- divotInside :: && (o in m.m.Keys);
+  //       assert forall o <- divotInside :: && (klonLine(o,m.m[o],m));
+  //
+  //       // assert forall o <- divotInside :: && (m.m[o] in rivetInside);  //ERR GRRR
+  //
+  //       assert divot.AMFO   >= pivot.AMFO;
+  //
+  //
+  //       assert forall d <- divotFringeNoPivot :: not(strictlyInside(d,pivot));
+  //       assert divotFringeNoPivot <= m.m.Keys;
+  //       assert forall d <- divotFringeNoPivot :: klonLine(d,m.m[d],m);
+  //       assert forall d <- divotFringeNoPivot :: m.m[d] == d;
 
- var rivetInside,rivetOutside,rivetFringe := splitOwnersAroundPivot(rivet, blivet);
- assert blivet in rivetFringe;
- var rivetFringeNoPivot := rivetFringe - {blivet};
-
-assert forall o <- divotInside :: && (o in m.m.Keys);
-assert forall o <- divotInside :: && (klonLine(o,m.m[o],m));
-
-// assert forall o <- divotInside :: && (m.m[o] in rivetInside);  //ERR GRRR
-
-assert divot.AMFO   >= pivot.AMFO;
-
-
-assert forall d <- divotFringeNoPivot :: not(strictlyInside(d,pivot));
-assert divotFringeNoPivot <= m.m.Keys;
-assert forall d <- divotFringeNoPivot :: klonLine(d,m.m[d],m);
-assert forall d <- divotFringeNoPivot :: m.m[d] == d;
-
-
-
-// assert forall d <- divotFringeNoPivot :: d in rivetFringeNoPivot;  //ERR GRRR
-// assert forall d <- rivetFringeNoPivot :: d in divotFringeNoPivot;  //ERR GRRR
-//
-// //  assert forall d <- divotInside :: m.m[d] in rivetInside;
-//  assert divotFringeNoPivot == rivetFringeNoPivot;                   //ERR GRRR
 
 
 
@@ -141,7 +134,7 @@ assert forall d <- divotFringeNoPivot :: m.m[d] == d;
 // }
 
 lemma SuperSplit(part : Object, pivot : Object, whole : Object)
-//part is sstrictly inside pivot AND so is whole (sob)
+  //part is sstrictly inside pivot AND so is whole (sob)
   requires part.Ready()
   requires pivot.Ready()
   requires whole.Ready()
@@ -149,40 +142,815 @@ lemma SuperSplit(part : Object, pivot : Object, whole : Object)
   requires strictlyInside(whole, pivot)
   requires inside(part, whole)
 {
-   var partInside,partOutside,partFringe    := splitOwnersAroundPivot(part, pivot);
-   var wholeInside,wholeOutside,wholeFringe := splitOwnersAroundPivot(whole, pivot);
+  var partInside,partOutside,partFringe    := splitOwnersAroundPivot(part, pivot);
+  var wholeInside,wholeOutside,wholeFringe := splitOwnersAroundPivot(whole, pivot);
 
-   assert part.AMFO   >= whole.AMFO;
-   assert partInside  >= wholeInside;
-   assert partOutside >= wholeOutside;  //seems odd, but remember ?outside? is the upwarads closure of owners beyond the pivot.
-   assert partFringe  >= wholeFringe;
+  assert part.AMFO   >= whole.AMFO;  //there it is????  this is it?
+  assert partInside  >= wholeInside;
+  assert partOutside >= wholeOutside;  //seems odd, but remember ?outside? is the upwarads closure of owners beyond the pivot.
+  assert partFringe  >= wholeFringe;
 }
 
 
-//
-// lemma superJoin(part : Object, pivot : Object, whole : Object,
-//                 partInside : Owner, partOutside : Owner, partFringe : Owner,
-//                 wholeInside : Owner, wholeOutside : Owner, wholeFringe : Owner)
-// ///likely unuseable, but...
-//   requires part.Ready()
-//   requires pivot.Ready()
-//   requires whole.Ready()
-//   requires AllReady(partInside)
-//   requires AllReady(partOutside)
-//   requires AllReady(partFringe)
-//   requires AllReady(wholeInside)
-//   requires AllReady(wholeOutside)
-//   requires AllReady(wholeFringe)
-//
-//
-//   requires strictlyInside(part, pivot)  //grr
-//   requires strictlyInside(whole, pivot) //grr
-//
-//    ensures inside(part, whole) //note not strictly
-// {}
 
-lemma splitOwnersAroundPivot(part : Object, pivot : Object) returns (allInside : Owner, allOutside : Owner, fringe : Owner)
-  //splits part.AMFO into the bits inside pivot,
+lemma farage(ownrs : OWNR, aliens : Owner)
+  //flattening anuthing within flatten(ownrs) is also in flatten(ownrs)bbb
+  requires AllReady((ownrs))
+  requires AllReady((aliens))
+  requires aliens <= flatten(ownrs)
+  ensures forall x : Object <- flatten(ownrs) :: x.AMFO <= flatten(ownrs)
+  ensures flatten(aliens) <= flatten(ownrs)
+{
+  var all := flatten(ownrs);
+  assert isFlat(all);
+  assert flatten(aliens) <= flatten(ownrs);
+}
+
+
+lemma farage3(ownrs : OWNR, othrs : OWNR, aliens : Owner)
+  requires AllReady((ownrs))
+  requires AllReady((othrs))
+  requires AllReady((aliens))
+  requires othrs <= ownrs
+  requires aliens <= flatten(ownrs)
+  ensures forall x : Object <- flatten(ownrs) :: x.AMFO <= flatten(ownrs)
+  ensures flatten(othrs)  <= flatten(ownrs)
+  ensures flatten(aliens) <= flatten(ownrs)
+{
+  var all := flatten(ownrs);
+  assert isFlat(all);
+
+  //  assert forall o <- all, oo <- o.AMFO :: oo in all;
+  //  assert forall o <- all, oo <- o.AMFO :: oo.AMFO <= all;
+  //  assert forall o <- all, oo <- o.AMFO, ooo <- oo.AMFO :: oo in all;
+  //  assert forall o <- all, oo <- o.AMFO, ooo <- oo.AMFO :: oo.AMFO <= all;
+  //  assert forall o <- all, oo <- o.AMFO, ooo <- oo.AMFO :: ooo in all;
+  //  assert forall o <- all, oo <- o.AMFO, ooo <- oo.AMFO :: ooo.AMFO <= all;
+
+  assert forall x : Object <- all :: x.AMFO <= all;
+
+  assert flatten(othrs)  <= flatten(ownrs);
+  assert flatten(aliens) <= flatten(ownrs);
+
+}
+
+
+lemma {:timeLimit 30} makersfield(ownrs : OWNR, pivot : Object)
+  requires AllReady(flatten(ownrs))
+  requires pivot.Ready()
+  ensures forall x <- ownrs ::    (x.AMFO >= pivot.AMFO) != (not(x.AMFO >= pivot.AMFO))
+  ensures forall x <- ownrs :: not(x.AMFO >= pivot.AMFO) != not(not(x.AMFO >= pivot.AMFO))
+  ensures forall x <- ownrs ::          outside(x,pivot) != not(outside(x,pivot))
+  ensures forall x <- ownrs ::           inside(x,pivot) != not( inside(x,pivot))
+{}
+
+// lemma SplitAround(oo : Owner, pivot : Object) returns (sinn : Owner, sout : Owner)
+//    requires AllReady(flatten(oo))
+//    requires pivot.Ready()
+//     ensures sinn == set o <- oo |    o.AMFO > pivot.AMFO
+//     ensures sout == set o <- oo | !( o.AMFO > pivot.AMFO )
+//     ensures forall o <- oo :: o in sinn || o in sout || o == pivot
+//     ensures sinn !! sout !! {pivot}
+//     ensures sinn+{pivot} == set o <- oo |    o.AMFO >= pivot.AMFO
+//     ensures sout+{pivot} == set o <- oo |  !( o.AMFO > pivot.AMFO )
+// {
+//   sinn := set o <- oo |    o.AMFO > pivot.AMFO;
+//   sout := set o <- oo | !( o.AMFO > pivot.AMFO );
+// }
+
+
+
+//{:timeLimit 30}
+lemma BROKEN_insidesFlattenFringe(ownrs : OWNR, pivot : Object) returns (allInside : Owner, allOutside : Owner, fringe : Owner)
+  //splits all into the bits inside pivot,
+  //the bits outside pivot,
+  //and the fringe (bits outside that are direct owners of an owner inside...)
+  //FUCK,. shoudl this be a function?  or indeed series of functions?
+  requires AllReady(flatten(ownrs))
+  requires pivot.Ready()
+
+  requires forall o <- ownrs :: strictlyInside(o, pivot)
+  requires ownrs > {}
+
+  ensures AllReady(allInside)
+  ensures AllReady(allOutside)
+  ensures AllReady(fringe)
+
+  ensures allInside  == set x <- flatten(ownrs) | strictlyInside(x, pivot)
+  ensures allOutside == set x <- flatten(ownrs) | not(strictlyInside(x, pivot))
+  ensures fringe == set x <- allInside, xo <- x.owner | (xo in allOutside) :: xo
+
+  ensures allInside + flatten(fringe) == flatten(ownrs)
+{
+  allInside  := set x <- flatten(ownrs) | strictlyInside(x, pivot);
+  allOutside := set x <- flatten(ownrs) | not(strictlyInside(x, pivot));
+  fringe := set x <- allInside, xo <- x.owner | (xo in allOutside)  :: xo;
+
+  // assert AIX: allInside  == set x <- flatten(ownrs) | strictlyInside(x, pivot);
+  // assert AOX: allOutside == set x <- flatten(ownrs) | not(strictlyInside(x, pivot));
+  // assert AFX: fringe == set x <- allInside, xo <- x.owner | (xo in allOutside) :: xo;
+
+  assert allInside != {};
+
+  assert flatten(ownrs) == allInside + allOutside;
+
+  assert fringe <= allOutside;
+  assert flatten(fringe) <= allOutside;
+  FlattenContainsFlatten(ownrs,fringe);
+  assert flatten(fringe) >= flatten(ownrs);
+  assert flatten(fringe)  == allOutside;
+
+  assert allInside + flatten(fringe) == flatten(ownrs);
+
+}
+
+
+
+function fOutside(ownrs : OWNR, pivot : Object) : (rv : Owner)
+  requires AllReady(flatten(ownrs))
+  requires pivot.Ready()
+  ensures AllReady(rv)
+{ set x <- flatten(ownrs) | not(strictlyInside(x, pivot)) }
+
+function fInside(ownrs : OWNR, pivot : Object) : (rv : Owner)
+  requires AllReady(flatten(ownrs))
+  requires pivot.Ready()
+  ensures AllReady(rv)
+{ set x <- flatten(ownrs) | (strictlyInside(x, pivot)) }
+
+function fFringe(ownrs : OWNR, pivot : Object) : (rv : Owner)
+  requires AllReady(flatten(ownrs))
+  requires pivot.Ready()
+  ensures AllReady(rv)
+{ set x <- fInside(ownrs,pivot), xo <- x.owner | (xo in fOutside(ownrs,pivot)) :: xo }
+
+
+function fFringe3(iwnrs : OWNR,  ownrs : OWNR, pivot : Object) : (rv : Owner)
+  requires AllReady(flatten(iwnrs))
+  requires AllReady(flatten(ownrs))
+  requires pivot.Ready()
+   ensures AllReady(rv)
+{ set x <- fInside(iwnrs,pivot), xo <- x.owner | (xo in fOutside(ownrs,pivot)) :: xo }
+
+
+
+lemma INSIDE_OUTSIDE(ownrs : OWNR, pivot : Object)
+  requires AllReady(flatten(ownrs))
+  requires pivot.Ready()
+  ensures flatten(ownrs) == (fInside(ownrs,pivot) + fOutside(ownrs,pivot))
+{}
+//    opaque {
+//         assert all == (allInside + allOutside);
+//         assert forall x <- allOutside :: not(strictlyInside(x, pivot));
+//         assert allOutside == all - allInside;
+//         assert pivot in allOutside;
+//
+//         assert forall x : Object <- all :: x.AMFO <= all;
+//         assert forall x <- allInside :: x.AMFO <= all;
+//         assert forall x <- allOutside :: x.AMFO <= all;
+//
+//         assert forall x <- all :: strictlyInside(x, pivot) != not(strictlyInside(x, pivot));
+//         assert allInside !! allOutside;
+//
+//         assert fringe <= allOutside;
+//
+//    }
+
+
+
+
+
+
+
+
+
+//{:timeLimit 30}   {:timeLimit 60} {:timeLimit 120}
+lemma  shouldBeSleeping(ownrs : OWNR, pivot : Object) returns (onnsiders : Owner, offsiders : Owner, allInside : Owner, allOutside : Owner, fringe : Owner)
+  //splits all into the bits inside pivot,
+  //the bits outside pivot,
+  //and the fringe (bits outside that are direct owners of an owner inside...)
+  //FUCK,. shoudl this be a function?  or indeed series of functions?
+  requires AllReady(flatten(ownrs))
+  requires pivot.Ready()     requires piR: pivot.Ready()
+
+
+///MISTAKE??   requires ownrs > pivot.AMFO  //the catch here is that it is possible x in ownrs but not(inside(x,pivot))
+  //say8ng exists x : strictlyInside(x,pivot) is anaother option...
+  //also; making oaners > pivot,AMFO is on reflection, clearly WRONG.,
+
+  ensures AllReady(allInside)
+  ensures AllReady(allOutside)
+  ensures AllReady(fringe)
+
+
+  //  ensures allOutside == set x <- flatten(ownrs) | not(strictlyInside(x, pivot))
+  //  ensures allInside !! allOutside
+  //  ensures flatten(ownrs) == (allInside + allOutside)
+  //  ensures fringe == set x <- allInside, xo <- x.owner | (xo in allOutside)  :: xo
+  //  ensures fringe <= allOutside
+
+
+
+
+  //    ensures (allInside > {}) ==> (flatten(fringe) == allOutside)    //ERR
+  //    ensures (allInside > {}) ==> (pivot in fringe)
+  //
+  //    ensures (fringe - {pivot}) == set x <- allInside, xo <- x.owner | (xo in allOutside) && (xo != pivot) :: xo    //ERR
+  //    ensures flatten(fringe - {pivot}) + flatten({pivot}) == flatten(fringe) == allOutside                        //ERR
+
+{
+  if (forall o <- ownrs :: not(strictlyInside(o, pivot)))
+  {
+    allInside := {};  allOutside := flatten(ownrs); fringe := {}; return;
+    //a more dedicated model could do more here, but not needed for correctness
+  }
+
+
+  onnsiders, offsiders := SplitTheDeadOwners(ownrs, pivot);
+
+  assert sonn: onnsiders == set x <- ownrs |  inside(x, pivot);
+  assert soff: offsiders == set x <- ownrs | outside(x, pivot);
+  assert summ: ownrs == offsiders + onnsiders;
+
+
+
+  var all := flatten(onnsiders);
+  allInside  := fInside(onnsiders,pivot);
+  allOutside := fOutside(onnsiders,pivot);
+  fringe := fFringe(onnsiders,pivot);
+
+  INSIDE_OUTSIDE(onnsiders, pivot);
+
+  var probe :|  probe in  fInside(onnsiders,pivot);
+  // assert (probe.AMFO > pivot.AMFO);
+  // assert (probe in allInside);
+
+  PivotInFringe(ownrs, pivot, probe);
+
+  farage(ownrs, {probe});
+  assert probe.AMFO <= all;
+
+
+  farage(ownrs, allOutside);
+  assert flatten(allOutside) <= all;
+
+
+  //
+  // // assert forall t <- allOutside :: t.AM551t                                           ot(strictlyInside(t, pivot));
+  //     ///THIS IS WRONG WERONG WONGO WRONG assert forall t <- allOutside, i <- allInside :: strictlyInside(i,t);
+  //
+  // assert  forall t <- allOutside, i <- allInside ::  strictlyInside(i,t) ==> t in i.AMFO;
+  // assert  forall t <- allOutside, i <- allInside ::  inside(i,t) ==> t in i.AMFO;
+  // assert  forall t <- allOutside, i <- allInside ::  inside(i,t) ==> t in flatten({i});
+  //
+  // // assert  forall t <- all        :: exists  o <- ownrs :: inside(t,o);
+  // // assert  forall t <- all        :: exists  o <- ownrs :: t in flatten({o});
+  // // assert forall t <- all  ::  flatten(ownrs)
+  //
+  // assert  forall t <- all        :: exists  o <- ownrs :: t in o.AMFO;
+  // assert  forall t <- allInside  :: exists  o <- ownrs :: t in o.AMFO;
+  // assert  forall t <- allOutside :: exists  o <- ownrs :: t in o.AMFO;
+  //
+  // //????assert  forall t <- allOutside, o <- ownrs :: strictlyInside(o,pivot) && t in flatten({o});
+  // //
+  // //
+  // //   forall t <- allOutside, i <- allInside
+  // //      |  strictlyInside(i,t) //&& strictlyInside(i,pivot) // && not(strictlyInside(t, pivot))
+  // //       ensures (t in flatten(fringe))
+  // //   {
+  // //       var prev, next := AcrossTheBorder(i, pivot, t); //TODO TODO TODO
+  // //       assert strictlyInside(prev,t);
+  // //       assert not(strictlyInside(next,pivot));
+  // //       assert prev in all;
+  // //       assert next in prev.owner;
+  // //       assert prev in allInside;
+  // //       assert next in allOutside;
+  // //       assert next in fringe;
+  // //       assert t in all;
+  // //       assert t in next.AMFO;
+  // //       assert t in flatten({next});
+  // //   }
+  // //
+
+  var fringeNoPivot:= fringe - {pivot};
+  assert pivot !in fringeNoPivot;
+
+  var flatFringeNoPivot := flatten(fringeNoPivot);
+
+  Notin(ownrs, pivot, allInside, allOutside, fringe);
+
+  //////////////////////////////////////////////////////////////////////////////
+
+  assert pivot !in flatten(fringe - {pivot});
+  assert pivot !in flatFringeNoPivot; //ERR
+
+
+
+
+
+  // assert fringe == set x <- allInside, xo <- x.owner | (xo in allOutside) :: xo  by { reveal AFX; }
+  //   assert fringeNoPivot == set x <- allInside, xo <- x.owner | (xo in allOutside) && (xo != pivot) :: xo;
+  //  //ERR
+  //   assert (fringe - {pivot}) == set x <- allInside, xo <- x.owner | (xo in allOutside) && (xo != pivot) :: xo;
+
+  FLATTEN_SUBS(fringe, {pivot});
+  assert flatten(fringe - {pivot}) + flatten({pivot}) == flatten(fringe); // == allOutside;
+
+  // assert allOutside == set x <- flatten(ownrs) | not(strictlyInside(x, pivot)) by { reveal AOX; }
+  // assert allInside  == set x <- flatten(ownrs) | strictlyInside(x, pivot) by { reveal AIX; }
+  // assert fringe == set x <- allInside, xo <- x.owner | (xo in allOutside) :: xo  by { reveal AFX; }
+  // assert  (allInside > {}) ==> (flatten(fringe) == allOutside);
+
+  // // // // // // // // // // // // // // // // // // // // // // // // // // // // // // // // // // // // // // // //
+  // // // // // // // // // // // // // // // // // // // // // // // // // // // // // // // // // // // // // // // //
+
+
+
+
+///GOLLUM assert forall x <- ownrs :: (x.AMFO >= pivot.AMFO) != not(x.AMFO >= pivot.AMFO); //ERR
+///GOLLUM assert forall x <- ownrs :: (outside(x, pivot) != not(outside(x, pivot)));       //ERR
+
+  //
+  // assert ownrs == offsiders + onnsiders;   //WZAEMMES
+  // assert flatten(ownrs) == (flatten(offsiders) + flatten(onnsiders));              //ERR
+  // assert offsiders !! onnsiders;
+  //
+
+
+
+
+
+
+
+
+
+assert forall o <- offsiders :: o in allOutside;
+assert forall o : Object <- offsiders :: o.AMFO <= allOutside;
+assert flatten(offsiders) <= allOutside;
+assert allInside <= flatten(onnsiders) <= all;
+
+assert forall f <- offsiders, x <- f.AMFO :: x in allOutside;
+assert fInside(offsiders, pivot) ==  {};
+assert fFringe(offsiders, pivot) ==  {};
+assert fInside(onnsiders+offsiders, pivot) ==  fInside(onnsiders,pivot);
+assert (onnsiders+offsiders) == ownrs by { reveal summ; }
+assert fInside(ownrs, pivot) == fInside(onnsiders, pivot);
+
+assert (set x <- fInside(ownrs,pivot), xo <- x.owner | (xo in fOutside(ownrs,pivot)) :: xo)
+          == fFringe3(ownrs, ownrs, pivot)
+          == fFringe(ownrs, pivot);
+
+//assert fFringe3(ownrs, ownrs, pivot) == fInside(ownrs, pivot);
+assert fFringe3(ownrs, ownrs, pivot)     == fFringe3(onnsiders, ownrs, pivot);
+///assert fFringe3(onnsiders, ownrs, pivot) >= fFringe3(onnsiders, onnsiders, pivot);
+
+// assert fFringe(ownrs, pivot) == fFringe(onnsiders, pivot);
+
+
+// opaque { assert fringe == set x <- fInside(ownrs,pivot), xo <- x.owner     | (xo in fOutside(onnsiders,pivot)) :: xo; }
+// opaque {  assert fringe == set x <- fInside(ownrs,pivot), xo <- x.owner     | (xo in fOutside(ownrs,pivot)) :: xo; }
+// opaque {  assert fringe == set x <- fInside(onnsiders,pivot), xo <- x.owner | (xo in fOutside(ownrs,pivot)) :: xo; }
+// opaque {  assert fringe == set x <- fInside(onnsiders,pivot), xo <- x.owner | (xo in fOutside(onnsiders,pivot)) :: xo; }
+
+
+  assert flatten(ownrs) == flatten(onnsiders) + flatten(offsiders) by
+   {  reveal sonn, soff, summ;
+      assert onnsiders + offsiders == ownrs;
+    FLATTEN_SUM3(onnsiders,offsiders,ownrs); }    //but not necessarily disjoint
+
+  assert fInside(ownrs, pivot) == fInside(onnsiders, pivot) + fInside(offsiders, pivot);
+  assert fFringe(ownrs, pivot) == fFringe(onnsiders, pivot) + fFringe(offsiders, pivot);
+
+
+forall f <- offsiders ensures (forall x <- f.AMFO :: outside(x,pivot)) {
+        FlattenOutsideFlatten(f,pivot);
+}
+
+
+
+
+  assert forall x <- fInside(ownrs,pivot), xo <- x.owner  :: xo in flatten(ownrs);
+
+//   assert fFringe(ownrs, pivot) == fFringe(onnsiders, pivot);
+
+
+ var onnInside, onnOutside, onnFringe := FlattenFringeIsAllOutside(onnsiders, pivot);
+
+assert allInside + flatten(fringe) == flatten(onnsiders);
+assert flatten(onnsiders) + flatten(offsiders) == flatten(ownrs);
+
+
+
+assert flatten(ownrs) == allInside + allOutside;
+
+assert flatten(ownrs) == fInside(ownrs,pivot) +  fOutside(ownrs,pivot);
+assert flatten(ownrs) == fInside(onnsiders,pivot) +  fOutside(ownrs,pivot);
+assert flatten(ownrs) == fInside(onnsiders,pivot) +  fOutside(ownrs,pivot);
+
+//lassert fOutside(ownrs,pivot) == flatten(fFringe(ownrs,pivot)) + flatten(offsiders);
+assert flatten(ownrs) == fInside(onnsiders,pivot) + flatten(fFringe(ownrs,pivot)) + flatten(offsiders);
+
+
+  assert allOutside == set x <- flatten(ownrs) | not(strictlyInside(x, pivot));
+  assert allInside == set x <- flatten(ownrs) | strictlyInside(x, pivot);
+  assert fringe == set x <- allInside, xo <- x.owner | (xo in allOutside) :: xo;
+}
+
+
+
+
+//{:timeLimit 30}   {:timeLimit 60} {:timeLimit 120}
+lemma {:timeLimit 120} splitOWNRSroundPivot(ownrs : OWNR, pivot : Object) returns (allInside : Owner, allOutside : Owner, fringe : Owner)
+  //splits all into the bits inside pivot,
+  //the bits outside pivot,
+  //and the fringe (bits outside that are direct owners of an owner inside...)
+  //FUCK,. shoudl this be a function?  or indeed series of functions?
+  requires AllReady(flatten(ownrs))
+  requires pivot.Ready()     requires piR: pivot.Ready()
+
+
+///MISTAKE??   requires ownrs > pivot.AMFO  //the catch here is that it is possible x in ownrs but not(inside(x,pivot))
+  //say8ng exists x : strictlyInside(x,pivot) is anaother option...
+  //also; making oaners > pivot,AMFO is on reflection, clearly WRONG.,
+
+  ensures AllReady(allInside)
+  ensures AllReady(allOutside)
+  ensures AllReady(fringe)
+
+  //  ensures allOutside == set x <- flatten(ownrs) | not(strictlyInside(x, pivot))
+  //  ensures allInside !! allOutside
+  //  ensures flatten(ownrs) == (allInside + allOutside)
+  //  ensures fringe == set x <- allInside, xo <- x.owner | (xo in allOutside)  :: xo
+  //  ensures fringe <= allOutside
+
+
+
+
+  //    ensures (allInside > {}) ==> (flatten(fringe) == allOutside)    //ERR
+  //    ensures (allInside > {}) ==> (pivot in fringe)
+  //
+  //    ensures (fringe - {pivot}) == set x <- allInside, xo <- x.owner | (xo in allOutside) && (xo != pivot) :: xo    //ERR
+  //    ensures flatten(fringe - {pivot}) + flatten({pivot}) == flatten(fringe) == allOutside                        //ERR
+
+{
+  if (forall o <- ownrs :: not(strictlyInside(o, pivot)))
+  {
+    allInside := {};  allOutside := flatten(ownrs); fringe := {}; return;
+    //a more dedicated model could do more here, but not needed for correctness
+  }
+
+  var all := flatten(ownrs);
+  allInside  := fInside(ownrs,pivot);
+  allOutside := fOutside(ownrs,pivot);
+  fringe := fFringe(ownrs,pivot);
+
+  INSIDE_OUTSIDE(ownrs, pivot);
+
+
+
+  //   assert exists x <- allInside :: (x.AMFO > pivot.AMFO) && (x.Ready());   //cos we know theere is something in AllInside or we'd have quit.
+
+  var probe :|  probe in  fInside(ownrs,pivot);
+  // assert (probe.AMFO > pivot.AMFO);
+  // assert (probe in allInside);
+
+  PivotInFringe(ownrs, pivot, probe);
+
+  farage(ownrs, {probe});
+  assert probe.AMFO <= all;
+
+
+  farage(ownrs, allOutside);
+  assert flatten(allOutside) <= all;
+
+
+  //
+  // // assert forall t <- allOutside :: t.AM551t                                           ot(strictlyInside(t, pivot));
+  //     ///THIS IS WRONG WERONG WONGO WRONG assert forall t <- allOutside, i <- allInside :: strictlyInside(i,t);
+  //
+  // assert  forall t <- allOutside, i <- allInside ::  strictlyInside(i,t) ==> t in i.AMFO;
+  // assert  forall t <- allOutside, i <- allInside ::  inside(i,t) ==> t in i.AMFO;
+  // assert  forall t <- allOutside, i <- allInside ::  inside(i,t) ==> t in flatten({i});
+  //
+  // // assert  forall t <- all        :: exists  o <- ownrs :: inside(t,o);
+  // // assert  forall t <- all        :: exists  o <- ownrs :: t in flatten({o});
+  // // assert forall t <- all  ::  flatten(ownrs)
+  //
+  // assert  forall t <- all        :: exists  o <- ownrs :: t in o.AMFO;
+  // assert  forall t <- allInside  :: exists  o <- ownrs :: t in o.AMFO;
+  // assert  forall t <- allOutside :: exists  o <- ownrs :: t in o.AMFO;
+  //
+  // //????assert  forall t <- allOutside, o <- ownrs :: strictlyInside(o,pivot) && t in flatten({o});
+  // //
+  // //
+  // //   forall t <- allOutside, i <- allInside
+  // //      |  strictlyInside(i,t) //&& strictlyInside(i,pivot) // && not(strictlyInside(t, pivot))
+  // //       ensures (t in flatten(fringe))
+  // //   {
+  // //       var prev, next := AcrossTheBorder(i, pivot, t); //TODO TODO TODO
+  // //       assert strictlyInside(prev,t);
+  // //       assert not(strictlyInside(next,pivot));
+  // //       assert prev in all;
+  // //       assert next in prev.owner;
+  // //       assert prev in allInside;
+  // //       assert next in allOutside;
+  // //       assert next in fringe;
+  // //       assert t in all;
+  // //       assert t in next.AMFO;
+  // //       assert t in flatten({next});
+  // //   }
+  // //
+
+  var fringeNoPivot:= fringe - {pivot};
+  assert pivot !in fringeNoPivot;
+
+  var flatFringeNoPivot := flatten(fringeNoPivot);
+
+  Notin(ownrs, pivot, allInside, allOutside, fringe);
+
+  //////////////////////////////////////////////////////////////////////////////
+
+  assert pivot !in flatten(fringe - {pivot});
+  assert pivot !in flatFringeNoPivot; //ERR
+
+
+
+
+
+  // assert fringe == set x <- allInside, xo <- x.owner | (xo in allOutside) :: xo  by { reveal AFX; }
+  //   assert fringeNoPivot == set x <- allInside, xo <- x.owner | (xo in allOutside) && (xo != pivot) :: xo;
+  //  //ERR
+  //   assert (fringe - {pivot}) == set x <- allInside, xo <- x.owner | (xo in allOutside) && (xo != pivot) :: xo;
+
+  FLATTEN_SUBS(fringe, {pivot});
+  assert flatten(fringe - {pivot}) + flatten({pivot}) == flatten(fringe); // == allOutside;
+
+  // assert allOutside == set x <- flatten(ownrs) | not(strictlyInside(x, pivot)) by { reveal AOX; }
+  // assert allInside  == set x <- flatten(ownrs) | strictlyInside(x, pivot) by { reveal AIX; }
+  // assert fringe == set x <- allInside, xo <- x.owner | (xo in allOutside) :: xo  by { reveal AFX; }
+  // assert  (allInside > {}) ==> (flatten(fringe) == allOutside);
+
+  // // // // // // // // // // // // // // // // // // // // // // // // // // // // // // // // // // // // // // // //
+  // // // // // // // // // // // // // // // // // // // // // // // // // // // // // // // // // // // // // // // //
+
+  var onnsiders, offsiders := SplitTheDeadOwners(ownrs, pivot);
+
+  assert sonn: onnsiders == set x <- ownrs |  inside(x, pivot);
+  assert soff: offsiders == set x <- ownrs | outside(x, pivot);
+  assert summ: ownrs == offsiders + onnsiders;
+
+
+  // makersfield(ownrs, pivot);
+
+///GOLLUM assert forall x <- ownrs :: (x.AMFO >= pivot.AMFO) != not(x.AMFO >= pivot.AMFO); //ERR
+///GOLLUM assert forall x <- ownrs :: (outside(x, pivot) != not(outside(x, pivot)));       //ERR
+
+  //
+  // assert ownrs == offsiders + onnsiders;   //WZAEMMES
+  // assert flatten(ownrs) == (flatten(offsiders) + flatten(onnsiders));              //ERR
+  // assert offsiders !! onnsiders;
+  //
+
+
+
+
+
+
+
+
+
+assert forall o <- offsiders :: o in allOutside;
+assert forall o : Object <- offsiders :: o.AMFO <= allOutside;
+assert flatten(offsiders) <= allOutside;
+assert allInside <= flatten(onnsiders) <= all;
+
+assert forall f <- offsiders, x <- f.AMFO :: x in allOutside;
+assert fInside(offsiders, pivot) ==  {};
+assert fFringe(offsiders, pivot) ==  {};
+assert fInside(onnsiders+offsiders, pivot) ==  fInside(onnsiders,pivot);
+assert (onnsiders+offsiders) == ownrs by { reveal summ; }
+assert fInside(ownrs, pivot) == fInside(onnsiders, pivot);
+
+assert (set x <- fInside(ownrs,pivot), xo <- x.owner | (xo in fOutside(ownrs,pivot)) :: xo)
+          == fFringe3(ownrs, ownrs, pivot)
+          == fFringe(ownrs, pivot);
+
+//assert fFringe3(ownrs, ownrs, pivot) == fInside(ownrs, pivot);
+assert fFringe3(ownrs, ownrs, pivot)     == fFringe3(onnsiders, ownrs, pivot);
+///assert fFringe3(onnsiders, ownrs, pivot) >= fFringe3(onnsiders, onnsiders, pivot);
+
+// assert fFringe(ownrs, pivot) == fFringe(onnsiders, pivot);
+
+
+// opaque { assert fringe == set x <- fInside(ownrs,pivot), xo <- x.owner     | (xo in fOutside(onnsiders,pivot)) :: xo; }
+// opaque {  assert fringe == set x <- fInside(ownrs,pivot), xo <- x.owner     | (xo in fOutside(ownrs,pivot)) :: xo; }
+// opaque {  assert fringe == set x <- fInside(onnsiders,pivot), xo <- x.owner | (xo in fOutside(ownrs,pivot)) :: xo; }
+// opaque {  assert fringe == set x <- fInside(onnsiders,pivot), xo <- x.owner | (xo in fOutside(onnsiders,pivot)) :: xo; }
+
+
+  assert flatten(ownrs) == flatten(onnsiders) + flatten(offsiders) by
+   {  reveal sonn, soff, summ;
+      assert onnsiders + offsiders == ownrs;
+    FLATTEN_SUM3(onnsiders,offsiders,ownrs); }    //but not necessarily disjoint
+
+  assert fInside(ownrs, pivot) == fInside(onnsiders, pivot) + fInside(offsiders, pivot);
+  assert fFringe(ownrs, pivot) == fFringe(onnsiders, pivot) + fFringe(offsiders, pivot);
+
+
+forall f <- offsiders ensures (forall x <- f.AMFO :: outside(x,pivot)) {
+        FlattenOutsideFlatten(f,pivot);
+}
+
+
+
+
+  assert forall x <- fInside(ownrs,pivot), xo <- x.owner  :: xo in flatten(ownrs);
+
+//   assert fFringe(ownrs, pivot) == fFringe(onnsiders, pivot);
+
+
+ var onnInside, onnOutside, onnFringe := FlattenFringeIsAllOutside(onnsiders, pivot);
+
+assert allInside + flatten(fringe) == flatten(onnsiders);
+assert flatten(onnsiders) + flatten(offsiders) == flatten(ownrs);
+
+
+
+assert flatten(ownrs) == allInside + allOutside;
+
+assert flatten(ownrs) == fInside(ownrs,pivot) +  fOutside(ownrs,pivot);
+assert flatten(ownrs) == fInside(onnsiders,pivot) +  fOutside(ownrs,pivot);
+assert flatten(ownrs) == fInside(onnsiders,pivot) +  fOutside(ownrs,pivot);
+
+//lassert fOutside(ownrs,pivot) == flatten(fFringe(ownrs,pivot)) + flatten(offsiders);
+assert flatten(ownrs) == fInside(onnsiders,pivot) + flatten(fFringe(ownrs,pivot)) + flatten(offsiders);
+
+
+  assert allOutside == set x <- flatten(ownrs) | not(strictlyInside(x, pivot));
+  assert allInside == set x <- flatten(ownrs) | strictlyInside(x, pivot);
+  assert fringe == set x <- allInside, xo <- x.owner | (xo in allOutside) :: xo;
+}
+
+
+
+
+lemma SplitTheDeadOwners(ownrs : OWNR, pivot : Object) returns (onnsiders : Owner, offsiders : Owner)
+  requires AllReady(flatten(ownrs))
+  requires pivot.Ready()
+  ensures onnsiders == set x <- ownrs |  inside(x, pivot)
+  ensures offsiders == set x <- ownrs | outside(x, pivot)
+  ensures ownrs == offsiders + onnsiders
+  ensures ownrs - offsiders == onnsiders
+  ensures ownrs - onnsiders == offsiders
+  ensures offsiders !! onnsiders
+  ensures flatten(ownrs) == (flatten(offsiders) + flatten(onnsiders))
+  ensures flatten(ownrs) >=  flatten(offsiders)
+  ensures flatten(ownrs) >=  flatten(onnsiders)
+{
+  onnsiders := set x <- ownrs |  inside(x, pivot);
+  offsiders := set x <- ownrs | outside(x, pivot);  //outside df not inside.
+
+  makersfield(ownrs, pivot);
+
+///GOLLUM assert forall x <- ownrs :: (x.AMFO >= pivot.AMFO) != not(x.AMFO >= pivot.AMFO); //ERR
+///GOLLUM assert forall x <- ownrs :: (outside(x, pivot) != not(outside(x, pivot)));       //ERR
+
+  assert ownrs == offsiders + onnsiders;
+  assert offsiders !! onnsiders;
+  assert flatten(ownrs) == (flatten(offsiders) + flatten(onnsiders));
+}
+
+lemma FlattenOutsideFlatten(sider : Object, pivot : Object)
+  requires sider.Ready()
+  requires pivot.Ready()
+  requires outside(sider,pivot)
+   ensures forall x <- sider.AMFO :: outside(x,pivot)
+{}
+
+
+lemma FlattenContainsFlatten(below : Owner, above : Owner)
+  requires AllReady(below)
+  requires AllReady(above)
+  requires flatten(below) >= above
+  ensures flatten(below) >= flatten(above)
+{
+  //  assert isFlat( flatten(below) );
+  //  assert forall o <- flatten(below), oo <- o.AMFO :: oo in flatten(below);
+  // assert forall o <- flatten(below) :: o.AMFO <= flatten(below);
+  //  assert forall a <- above :: a in flatten(below);
+  //   assert forall a <- above :: a.AMFO <= flatten(below);
+}
+
+
+lemma FlattenFringeIsAllOutside(iwnrs : OWNR,  pivot : Object) returns (allInside : Owner, allOutside : Owner, fringe : Owner)
+  //ensuress flatten(fringe) == allOutside
+  //all iwnrs must all be strictlyInside piot
+  //pretty much the wrong thing cons iwnrs != owners != ownrs != onnsiders...
+
+ requires forall i <- iwnrs :: strictlyInside(i, pivot)
+
+ requires AllReady(flatten(iwnrs))
+ requires pivot.Ready()
+
+  ensures allInside  == set x <- flatten(iwnrs) | strictlyInside(x, pivot)
+  ensures allOutside == set x <- flatten(iwnrs) | not(strictlyInside(x, pivot))
+  ensures allInside !! allOutside
+  ensures flatten(iwnrs) == (allInside + allOutside)
+  ensures fringe == set x <- allInside, xo <- x.owner | (xo in allOutside)  :: xo
+
+  ensures iwnrs <= allInside
+  ensures forall o <- allInside  :: o.owner <= (allInside + allOutside)
+  ensures forall o <- allOutside :: o.owner <= allOutside
+  ensures forall o <- allInside, oo <- o.owner ::  (oo in allOutside) == (oo in fringe)
+  ensures fringe <= allOutside
+  ensures flatten(fringe) == allOutside
+{
+
+  allInside  := set x <- flatten(iwnrs) | strictlyInside(x, pivot);
+  allOutside := set x <- flatten(iwnrs) | not(strictlyInside(x, pivot));
+  fringe := set x <- allInside, xo <- x.owner | (xo in allOutside)  :: xo;
+
+  assert fringe <= allOutside;
+  assert flatten(fringe) <= allOutside;
+
+  assert forall t <- allOutside :: t in flatten(iwnrs);
+
+  forall t <- allOutside ensures (t in flatten(fringe)) //(t in flatten(fringe))  //by
+  {
+    forall part <- iwnrs | (t in flatten({part})) ensures (t in flatten(fringe)) {
+      var prev, next := AcrossTheBorder(part, pivot, t);
+      assert strictlyInside(prev,t);
+      assert not(strictlyInside(next,pivot));
+      assert prev in flatten(iwnrs);
+      assert next in prev.owner;
+      assert prev in allInside;
+      assert next in allOutside;
+      assert next in fringe;
+      assert t in flatten(iwnrs);
+      assert t in next.AMFO;
+      assert t in flatten({next});
+      assert t in flatten(fringe);
+    }
+  }
+
+  assert flatten(fringe) >= allOutside;
+  assert flatten(fringe) == allOutside;
+
+}
+
+
+
+lemma OnlyThrough(ownrs : OWNR,  pivot : Object,  allInside : Owner, allOutside : Owner, fringe : Owner)
+  //proof by contradiction?
+  //to get from ownrs thru pivot to outside you must go through fringe x
+  requires AllReady(flatten(ownrs))
+  requires pivot.Ready()
+  requires allInside  == set x <- flatten(ownrs) | strictlyInside(x, pivot)
+  requires allOutside == set x <- flatten(ownrs) | not(strictlyInside(x, pivot))
+  requires allInside !! allOutside
+  requires flatten(ownrs) == (allInside + allOutside)
+  requires fringe == set x <- allInside, xo <- x.owner | (xo in allOutside)  :: xo
+  requires fringe <= allOutside
+  //requires (allInside > {}) ==> (flatten(fringe) == allOutside)
+  requires (allInside > {}) ==> (pivot in fringe)
+
+  ensures pivot !in flatten(fringe - {pivot})
+{
+  if (pivot in flatten(fringe - {pivot})) {
+    assert not(fringe <= allOutside);
+    assert false;
+  }
+}
+
+
+
+
+lemma Notin(ownrs : OWNR,  pivot : Object, allInside : Owner, allOutside : Owner, fringe : Owner)
+  //proof by contradiction
+  //pivot is not in rest of fringe
+  requires AllReady(flatten(ownrs))
+  // requires pivot.Ready()
+  requires allInside  == set x <- flatten(ownrs) | strictlyInside(x, pivot)
+  requires allOutside == set x <- flatten(ownrs) | not(strictlyInside(x, pivot))
+  // requires allInside !! allOutside
+  // requires flatten(ownrs) == (allInside + allOutside)
+  requires fringe == set x <- allInside, xo <- x.owner | (xo in allOutside)  :: xo
+  // requires fringe <= allOutside
+  //requires (allInside > {}) ==> (flatten(fringe) == allOutside)
+  //requires (allInside > {}) ==> (pivot in fringe)
+
+  ensures pivot !in flatten(fringe - {pivot})
+{
+  if (pivot in flatten(fringe - {pivot})) {
+    assert not(fringe <= allOutside);
+    assert false;
+  }
+}
+
+
+
+lemma {:resource_limit 70000000}  {:timeLimit 20} splitOwnersAroundPivot(part : Object, pivot : Object) returns (allInside : Owner, allOutside : Owner, fringe : Owner)
+  //splits all into the bits inside pivot,
   //the bits outside pivot,
   //and the fringe (bits outside that are direct owners of an owner inside...)
   //FUCK,. shoudl this be a function?  or indeed series of functions?
@@ -190,49 +958,49 @@ lemma splitOwnersAroundPivot(part : Object, pivot : Object) returns (allInside :
   requires pivot.Ready()
   requires strictlyInside(part, pivot)
 
-   ensures AllReady(allInside)
-   ensures AllReady(allOutside)
-   ensures AllReady(fringe)
+  ensures AllReady(allInside)
+  ensures AllReady(allOutside)
+  ensures AllReady(fringe)
 
-   ensures allInside  == set x <- part.AMFO | strictlyInside(x, pivot)
-   ensures allOutside == set x <- part.AMFO | not(strictlyInside(x, pivot))
-   ensures allInside !! allOutside
-   ensures part.AMFO == (allInside + allOutside)
-   ensures fringe == set x <- allInside, xo <- x.owner | (xo in allOutside)  :: xo
-   ensures forall x <- fringe :: x in allOutside
-   ensures flatten(fringe) == allOutside
-   ensures pivot in fringe
-   ensures (fringe - {pivot}) == set x <- allInside, xo <- x.owner | (xo in allOutside) && (xo != pivot) :: xo
-   ensures flatten(fringe - {pivot}) + flatten({pivot}) == flatten(fringe) == allOutside
+  ensures allInside  == set x <- part.AMFO | strictlyInside(x, pivot)
+  ensures allOutside == set x <- part.AMFO | not(strictlyInside(x, pivot))
+  ensures allInside !! allOutside
+  ensures part.AMFO == (allInside + allOutside)
+  ensures fringe == set x <- allInside, xo <- x.owner | (xo in allOutside)  :: xo
+  ensures forall x <- fringe :: x in allOutside
+  ensures flatten(fringe) == allOutside
+  ensures pivot in fringe
+  ensures (fringe - {pivot}) == set x <- allInside, xo <- x.owner | (xo in allOutside) && (xo != pivot) :: xo
+  ensures flatten(fringe - {pivot}) + flatten({pivot}) == flatten(fringe) == allOutside
 
-   //ensures part.AMFO == recOwners(part)  //can do with Axioms from Ownership-Parallel if necessary...
+  //ensures all == recOwners(part)  //can do with Axioms from Ownership-Parallel if necessary...
 
-  {
-   var all := part.AMFO;
+{
+  var all := part.AMFO;
 
-   allInside  := set x <- part.AMFO | strictlyInside(x, pivot);
-   assert part in allInside;
+  allInside  := set x <- all | strictlyInside(x, pivot);
+  assert part in allInside;
 
-   allOutside := part.AMFO - allInside;
-   assert forall x <- allOutside :: not(strictlyInside(x, pivot));
-   assert pivot in allOutside;
+  allOutside := all - allInside;
+  assert forall x <- allOutside :: not(strictlyInside(x, pivot));
+  assert pivot in allOutside;
 
-   assert forall x <- part.AMFO :: strictlyInside(x, pivot) != not(strictlyInside(x, pivot));
+  assert forall x <- all :: strictlyInside(x, pivot) != not(strictlyInside(x, pivot));
 
-   assert allInside !! allOutside;
-   assert all == (allInside + allOutside);
+  assert allInside !! allOutside;
+  assert all == (allInside + allOutside);
 
-   fringe := set x <- part.AMFO, xo <- x.owner | (x in allInside) && (xo in allOutside)  :: xo;
-   assert fringe <= allOutside;
-   assert fringe == set x <- allInside, xo <- x.owner | (xo in allOutside)  :: xo;
+  fringe := set x <- all, xo <- x.owner | (x in allInside) && (xo in allOutside)  :: xo;
+  assert fringe <= allOutside;
+  assert fringe == set x <- allInside, xo <- x.owner | (xo in allOutside)  :: xo;
 
-   assert part !in fringe;
-//   assert exists x <- allInside, xo <- x.owner ::  xo == pivot;
+  assert part !in fringe;
+  //   assert exists x <- allInside, xo <- x.owner ::  xo == pivot;
 
   var prev := YouGetThereEventually(part, pivot);
   assert pivot in prev.owner;
   assert strictlyInside(prev,pivot);
-  assert prev in part.AMFO;
+  assert prev in all;
   assert inside(part,prev);
   assert prev in allInside;
   assert pivot in allOutside;
@@ -245,17 +1013,17 @@ lemma splitOwnersAroundPivot(part : Object, pivot : Object) returns (allInside :
 
   forall t <- allOutside ensures (t in flatten(fringe)) //(t in flatten(fringe))  //by
   {
-      var prev, next := AcrossTheBorder(part, pivot, t);
-      assert strictlyInside(prev,t);
-      assert not(strictlyInside(next,pivot));
-      assert prev in part.AMFO;
-      assert next in prev.owner;
-      assert prev in allInside;
-      assert next in allOutside;
-      assert next in fringe;
-      assert t in part.AMFO;
-      assert t in next.AMFO;
-      assert t in flatten({next});
+    var prev, next := AcrossTheBorder(part, pivot, t);
+    assert strictlyInside(prev,t);
+    assert not(strictlyInside(next,pivot));
+    assert prev in all;
+    assert next in prev.owner;
+    assert prev in allInside;
+    assert next in allOutside;
+    assert next in fringe;
+    assert t in all;
+    assert t in next.AMFO;
+    assert t in flatten({next});
   }
 
   assert flatten(fringe) >= allOutside;
@@ -277,35 +1045,36 @@ lemma splitOwnersAroundPivot(part : Object, pivot : Object) returns (allInside :
 
 
 lemma AcrossTheBorder(part : Object,  pivot : Object, whole : Object) returns (prev : Object, next : Object)
-  //returns transitive owners of part that on the way to whole, where prev is inside pivot, and next is outside or == pivot
- decreases part.AMFO
+  //returns two transitive owners of part that on the way to whole, where prev is inside pivot, and next is outside or == pivot
+  decreases part.AMFO
   requires part.Ready()
   requires whole.Ready()
   requires strictlyInside(part, whole)
   requires strictlyInside(part, pivot)
   requires not(strictlyInside(whole, pivot))
 
-   ensures part != whole
-   ensures prev in part.AMFO
-   ensures next in part.AMFO
-   ensures inside(part,prev)
-   ensures strictlyInside(part,next)
-   ensures strictlyInside(prev,pivot)
-   ensures next in prev.owner
-   ensures not(strictlyInside(next,pivot))
-   ensures prev.Ready()
-   ensures next.Ready()
-   ensures whole in part.AMFO
-   ensures whole in flatten({next})
-   {
-    prev := part;
+  ensures part != whole
+  ensures prev in part.AMFO
+  ensures next in part.AMFO
+  ensures inside(part,prev)
+  ensures strictlyInside(part,next)
+  ensures strictlyInside(prev,pivot)
+  ensures strictlyInside(prev,whole)
+  ensures next in prev.owner
+  ensures not(strictlyInside(next,pivot))
+  ensures prev.Ready()
+  ensures next.Ready()
+  ensures whole in part.AMFO
+  ensures whole in flatten({next})
+{
+  prev := part;
 
-    if (whole in prev.owner) {
-        next := whole;
-        return;
-    }
+  if (whole in prev.owner) {
+    next := whole;
+    return;
+  }
 
-    next := YouCan'tGetThereFromHereBut(prev, whole);
+  next := YouCan'tGetThereFromHereBut(prev, whole);
 
   //  assert part != whole;
   //  assert prev in part.AMFO;
@@ -317,21 +1086,21 @@ lemma AcrossTheBorder(part : Object,  pivot : Object, whole : Object) returns (p
   //  assert prev.Ready();
   //  assert next.Ready();
 
-    while (strictlyInside(next,pivot))
-      decreases next.AMFO
-      invariant part != whole
-      invariant prev in part.AMFO
-      invariant next in part.AMFO
-      invariant next in prev.owner
-      invariant inside(part,prev)
-      invariant strictlyInside(prev,pivot)
-      invariant inside(next,whole)
-      invariant prev.Ready()
-      invariant next.Ready()
-    {
-      prev := next;
-      next := YouCan'tGetThereFromHereBut(prev, whole);
-    }
+  while (strictlyInside(next,pivot))
+    decreases next.AMFO
+    invariant part != whole
+    invariant prev in part.AMFO
+    invariant next in part.AMFO
+    invariant next in prev.owner
+    invariant inside(part,prev)
+    invariant strictlyInside(prev,pivot)
+    invariant inside(next,whole)
+    invariant prev.Ready()
+    invariant next.Ready()
+  {
+    prev := next;
+    next := YouCan'tGetThereFromHereBut(prev, whole);
+  }
 
   //  assert part != whole;
   //  assert prev in part.AMFO;
@@ -343,46 +1112,102 @@ lemma AcrossTheBorder(part : Object,  pivot : Object, whole : Object) returns (p
   //  assert prev.Ready();
   //  assert next.Ready();
 
-   }
+}
+
+
+
+
+lemma PivotInFringe(ownrs : OWNR, pivot : Object, probe : Object)
+  decreases probe.AMFO
+  requires AllReady(flatten(ownrs))
+
+  requires probe.Ready()
+  requires pivot.Ready()
+  requires strictlyInside(probe, pivot)
+  requires probe != pivot
+  requires exists o <- ownrs :: strictlyInside(o,pivot)
+
+   ensures pivot in fFringe(ownrs, pivot)
+{
+   var prev := YouGetThereEventually(probe, pivot);
+    assert pivot in prev.owner;
+    assert strictlyInside(prev,pivot);
+
+    assert prev  in fInside(ownrs, pivot);
+    assert pivot in fOutside(ownrs, pivot);
+    assert pivot in fFringe(ownrs, pivot);
+}
+
+
+
+lemma OwnerInFlatten(xwrns : OWNR, a : Object, b : Object)
+  requires AllReady(flatten(xwrns))
+  requires a.Ready()
+  requires b.Ready()
+
+  requires a in flatten(xwrns)
+  requires b in a.owner
+
+  ensures b in flatten(xwrns)
+{}
 
 
 
 
 lemma YouGetThereEventually(part : Object, whole : Object) returns (prev : Object)
- //returns a (transitive) owner of part that is JUST BEFORE whole --- ie of which whole is a direct owner
- decreases part.AMFO
+  //returns a (transitive) owner of part that is JUST BEFORE whole --- ie of which whole is a direct owner
+  decreases part.AMFO
   requires part.Ready()
   requires whole.Ready()
   requires strictlyInside(part, whole)
-   ensures part != whole
-   ensures prev in part.AMFO
-   ensures whole in prev.owner
-   ensures strictlyInside(prev,whole)
-   {
-    if (whole in part.owner) {
-        prev := part;
-        assert prev in part.AMFO && whole in prev.owner;
-        return;
-    }
+  ensures part != whole
+  ensures prev in part.AMFO
+  ensures whole in prev.owner
+  ensures strictlyInside(prev,whole)
+  ensures inside(part, prev)
+{
+  if (whole in part.owner) {
+    prev := part;
+    assert prev in part.AMFO && whole in prev.owner;
+    return;
+  }
   assert whole !in part.owner;
 
-    ThereIsALightThatNeverGoesOut(part, whole);
- //   assert (exists prev <- part.owner :: inside(prev, whole));
+  ThereIsALightThatNeverGoesOut(part, whole);
+  //   assert (exists prev <- part.owner :: inside(prev, whole));
 
-    prev := YouCan'tGetThereFromHereBut(part, whole);
-    assert prev in part.owner;   assert whole !in part.owner;     assert prev != whole;
-    assert inside(prev,whole);
+  prev := YouCan'tGetThereFromHereBut(part, whole);
+  assert prev in part.owner;   assert whole !in part.owner;     assert prev != whole;
+  assert inside(prev,whole);
 
-    if (whole in prev.owner) {
-        assert prev in part.AMFO && whole in prev.owner;
-        return;
-    }
-    prev := YouGetThereEventually(prev, whole);
-   }
+  if (whole in prev.owner) {
+    assert prev in part.AMFO && whole in prev.owner;
+    return;
+  }
+  prev := YouGetThereEventually(prev, whole);
+}
 
 
 // // // // // // // // // // // // // // // // // // // // // // // // // // // // // // // ////
 /// // // // // // // // // // // // // // // // // // // // // // // // // // // // // // // ///
+
+
+//
+// lemma {:timeLimit 30} LetMeBeYourLighthouseKeeper(below : OWNR, above : OWNR)
+//   //at least one of below's direct owners is on the way to above.
+//   requires AllReady(below) && isFlat(below)
+//   requires AllReady(above) && isFlat(above)
+//   requires below >= above
+//   ensures (below == above) || (exists x <- below :: x.AMFO >= above)
+//  {
+//     if (below == above) {
+//       assert ((below == above) || (exists x <- below :: x.AMFO >= above));
+//       return; }
+//
+//     assert below != above;
+//     assert (exists x <- below :: x.AMFO >= above);
+//  }
+
 
 
 //
@@ -392,50 +1217,48 @@ lemma {:timeLimit 30} ThereIsALightThatNeverGoesOut(part : Object, whole : Objec
   requires whole.Ready()
   requires inside(part,whole)
   ensures (part == whole) || (exists x <- part.owner :: inside(x, whole))
- {
-    InsideRecInside2(part, whole);
+{
+  //    InsideRecInside2(part, whole);
 
-    if (part == whole) {
-      assert ((part == whole) || (exists x <- part.owner :: inside(x, whole)));
-      return; }
+  if (part == whole) {
+    assert ((part == whole) || (exists x <- part.owner :: inside(x, whole)));
+    return; }
 
-    assert part != whole;
-    assert (exists x <- part.owner :: recInside(x,whole));
- }
+  assert part != whole;
+  assert (exists x <- part.owner :: inside(x,whole));
+}
 
 
 ghost function {:isolate_assertions} YouCan'tGetThereFromHereBut(part : Object, whole : Object) : (next : Object)
   //return next - a "direct owner" of part that is on the way up to "whole"
- decreases part.AMFO
+  decreases part.AMFO
 
   requires part.Ready()
   requires whole.Ready()
   requires part != whole
   requires inside(part,whole)
 
-   ensures next in part.owner
-   ensures strictlyInside(part, next)
-   ensures inside(next,whole)
-   ensures (part.AMFO decreases to next.AMFO)
-  {
-    InsideRecInside2(part, whole);
-    assert recInside(part, whole);
-    ThereIsALightThatNeverGoesOut(part, whole);
+  ensures next in part.owner
+  ensures strictlyInside(part, next)
+  ensures inside(next,whole)
+  ensures (part.AMFO decreases to next.AMFO)
+{
+  InsideRecInside2(part, whole);
+  assert recInside(part, whole);
+  ThereIsALightThatNeverGoesOut(part, whole);
 
-    assert exists x <- part.owner :: inside(x, whole);
+  assert exists x <- part.owner :: inside(x, whole);
 
-    var next : Object :| next in part.owner && inside(next, whole);
+  var next : Object :| next in part.owner && inside(next, whole);
 
-    assert part !in part.owner;
-    assert next  in part.owner;
-    assert part.AMFO > next.AMFO;
-    assert (part.AMFO decreases to next.AMFO);
-    assert inside(next,whole);
+  assert part !in part.owner;
+  assert next  in part.owner;
+  assert part.AMFO > next.AMFO;
+  assert (part.AMFO decreases to next.AMFO);
+  assert inside(next,whole);
 
-    next
-  }
-
-
+  next
+}
 
 
 
@@ -444,47 +1267,19 @@ ghost function {:isolate_assertions} YouCan'tGetThereFromHereBut(part : Object, 
 
 
 
- //  ensures pivotlyOutside(part, whole) == not(strictlyInside(part, whole))
 
-//    var allInside  := set x <- part.AMFO :: strictlyInside(x, whole);
-//    var allOutside := set x <- part.AMFO :: pivotlyOutside(x, whole);
-//
-//    if (strictlyInside(part, whole))
-//     {
-//         assert pivotlyOutside(part, whole) == not(strictlyInside(part, whole)); return;
-//     }
-//
-//   if (part == whole)
-//     {
-//         assert pivotlyOutside(part, whole) == not(strictlyInside(part, whole)); return;
-//     }
-//
-//   assert not(strictlyInside(part, whole));
-//   assert not(part.AMFO > whole.AMFO);
-//   assert part != whole;
-//   AXIOMAMFOS(part,whole);
-//   assert part.AMFO != whole.AMFO;
-//   assert not(part.AMFO >= whole.AMFO);
-//   assert not(inside(part, whole));
-//
-//   assert pivotlyOutside(part, whole) == not(strictlyInside(part, whole));
+lemma FLATTEN_SUBS(a : Owner, b : Owner)
+  requires a >= b
+  ensures flatten(a - b) + flatten(b) == flatten(a)
+{}
 
-lemma Flatten3(a : Owner, b : Owner, c : Owner)
-  // requires AllReady(a)
-  // requires AllReady(b)
-  // requires AllReady(c)
-  requires forall o <- a :: o.Ready()
-  requires forall o <- b :: o.Ready()
-  requires forall o <- c :: o.Ready()
-
-    requires a + b == c
-    ensures flatten(a) + flatten(b) == flatten(c)
-    ensures flatten(a) + flatten(b) == flatten(a+b)
-    ensures recFlatten(a)+recFlatten(b)==recFlatten(a+b)
-    {}
+lemma FLATTEN_SUM3(a : Owner, b : Owner, c : Owner)
+  requires a+b == c
+  ensures flatten(a) + flatten(b) == flatten(a+b)
+{}
 
 lemma FLATTEN_SUMS(a : Owner, b : Owner, c : Owner, m : Klon)
-   requires a+b == c
+  requires a+b == c
   // requires forall o <- a :: o.Ready()  //I'm OH SO TORY
   // requires forall o <- b :: o.Ready()  //I'm OH SO TORY
   // requires forall o <- c :: o.Ready()  //TORY TORY TORY
@@ -493,17 +1288,17 @@ lemma FLATTEN_SUMS(a : Owner, b : Owner, c : Owner, m : Klon)
   //  requires AllReady(c)
   //  requires klonReady(m)
   //  requires klonCalid(m)
-   requires (a+b+c) <= m.m.Keys
-//    ensures recFlatten(a)+recFlatten(b)==recFlatten(a+b)
-    ensures flatten(a) + flatten(b) == flatten(a+b)
-    ensures mapThruKlon(a,m) + mapThruKlon(b,m) == mapThruKlon(a+b,m)
-    ensures flatten(mapThruKlon(a,m)) + flatten(mapThruKlon(b,m)) == flatten(mapThruKlon(a+b,m))
-   {}
+  requires (a+b+c) <= m.m.Keys
+  //    ensures recFlatten(a)+recFlatten(b)==recFlatten(a+b)
+  ensures flatten(a) + flatten(b) == flatten(a+b)
+  ensures mapThruKlon(a,m) + mapThruKlon(b,m) == mapThruKlon(a+b,m)
+  ensures flatten(mapThruKlon(a,m)) + flatten(mapThruKlon(b,m)) == flatten(mapThruKlon(a+b,m))
+{}
 
 lemma FLATTEN_ONE(o : Object)
- requires o.Ready()
- ensures flatten({o}) == {o} + flatten(o.owner) == o.AMFO
- {}
+  requires o.Ready()
+  ensures flatten({o}) == {o} + flatten(o.owner) == o.AMFO
+{}
 
 
 lemma {:timeLimit 20} MAPPEN_ONE(next : Object, m : Klon)
@@ -511,12 +1306,12 @@ lemma {:timeLimit 20} MAPPEN_ONE(next : Object, m : Klon)
   requires next in m.m.Keys
   requires klonReady(m)
   requires klonCalid(m)
-   ensures mapThruKlon({next},m) == {m.m[next]}
-//   ensures flatten({next}) == {next} + flatten(next.owner)
-//   ensures flatten(mapThruKlon(done+{next},m)) == flatten(mapThruKlon(done,m)) + flatten(mapThruKlon({next},m))
+  ensures mapThruKlon({next},m) == {m.m[next]}
+  //   ensures flatten({next}) == {next} + flatten(next.owner)
+  //   ensures flatten(mapThruKlon(done+{next},m)) == flatten(mapThruKlon(done,m)) + flatten(mapThruKlon({next},m))
 {
-    FLATTEN_ONE(next);
-//  assert mapThruKlon({next},m) == (set o <- {next} :: m.m[o]) == {m.m[next]};
+  FLATTEN_ONE(next);
+  //  assert mapThruKlon({next},m) == (set o <- {next} :: m.m[o]) == {m.m[next]};
 }
 
 lemma {:timeLimit 20} FLATTEN_TWO(done : Owner, next : Object, m : Klon)
@@ -525,107 +1320,186 @@ lemma {:timeLimit 20} FLATTEN_TWO(done : Owner, next : Object, m : Klon)
   requires klonReady(m)
   requires klonCalid(m)
   requires (done+{next}) <= m.m.Keys
-   ensures (done+{next} == done + {next})
-   ensures mapThruKlon(done+{next},m) == mapThruKlon(done,m) + mapThruKlon({next},m)
-   ensures flatten(done+{next}) == flatten(done) + flatten({next})
-   ensures flatten(mapThruKlon(done+{next},m)) == flatten(mapThruKlon(done,m)) + flatten(mapThruKlon({next},m))
+  ensures (done+{next} == done + {next})
+  ensures mapThruKlon(done+{next},m) == mapThruKlon(done,m) + mapThruKlon({next},m)
+  ensures flatten(done+{next}) == flatten(done) + flatten({next})
+  ensures flatten(mapThruKlon(done+{next},m)) == flatten(mapThruKlon(done,m)) + flatten(mapThruKlon({next},m))
 {
   FLATTEN_SUMS(done,{next},done+{next},m);
 }
 
+// ghost function claudeSplatten(oo: Owner, m: Klon): Owner
+//      reads m.hns()
+//  decreases allAMFOs(oo)
+//   requires AllReady(oo)
+//   requires klonReady(m)
+//   requires klonCalid(m)
+//   requires oo <= m.m.Keys
+//   ensures flatten(oo) <= m.m.Keys
+//   ensures recSplatten(oo, m) == flatten(mapThruKlon(oo, m))
+// {
+//   if oo == {} then {}
+//   else
+//     var next :| next in oo;
+//     var sext := m.m[next];
+//     var fowner :=
+//       if next == m.o then flatten(m.clowner)
+//       else if outside(next, m.o) then flatten(next.owner)
+//       else recSplatten(next.owner, m);
+//       assert next in oo;
+//       assert allAMFOs(oo) decreases to allAMFOs(oo - {next});
+//     ({sext} + fowner) + recSplatten(oo - {next}, m)
+// }
+
+
+
+lemma OH_FUCK_WHAT_HAVE_I_DONE(oo : Owner, m : Klon) returns (sp : Owner)
+  decreases allAMFOs(oo)
+  requires AllReady(oo)
+  requires klonReady(m)
+  requires klonCalid(m)
+  requires oo <= m.m.Keys
+{
+  var rsp := recSplatten(oo,m);
+  var fmk := flatten(mapThruKlon(oo,m));
+  var mkf := mapThruKlon(flatten(oo),m);
+
+  assert rsp == fmk;
+  sp := oo;
+}
 
 
 
 lemma recSplatten(oo : Owner, m : Klon) returns (sp : Owner)
   decreases allAMFOs(oo)
-   requires AllReady(oo)
-   requires klonReady(m)
-   requires klonCalid(m)
-   requires oo <= m.m.Keys
-//
-//    requires |oo| == 1
-//    requires forall o <- oo :: o.owner == {}
-//     ensures flatten(oo) == oo
+  requires AllReady(oo)
+  requires klonReady(m)
+  requires klonCalid(m)
+  requires oo <= m.m.Keys
+  //
+  //    requires |oo| == 1
+  //    requires forall o <- oo :: o.owner == {}
+  //     ensures flatten(oo) == oo
 
-    ensures flatten(oo) <= m.m.Keys
-    ensures sp == flatten(mapThruKlon(oo, m))
-   {
-//     var x :=  {set o : Object <- oo, ooo <- recOwners(o) :: ooo};
+  ensures flatten(oo) <= m.m.Keys
+  ensures sp == flatten(mapThruKlon(oo, m))
+{
+  //     var x :=  {set o : Object <- oo, ooo <- recOwners(o) :: ooo};
 
-    sp := {};
+  sp := {};
 
-    var todo := oo;
-    var done : Owner := {};
-    assert AllReady(todo);
-    assert oo - todo == {};
-    assert mapThruKlon({}, m) == {};
-    assert mapThruKlon((oo - todo), m) == {};
-    assert flatten({}) == {};
-    assert flatten(mapThruKlon((oo - todo), m)) == {};
+  var todo := oo;
+  var done : Owner := {};
+  assert AllReady(todo);
+  assert oo - todo == {};
+  assert mapThruKlon({}, m) == {};
+  assert mapThruKlon((oo - todo), m) == {};
+  assert flatten({}) == {};
+  assert flatten(mapThruKlon((oo - todo), m)) == {};
 
+  assert sp == flatten(mapThruKlon((oo - todo), m));
+  assert done == oo - todo == {};
+  assert sp == flatten(mapThruKlon((done), m));
+
+  while (todo > {})
+    decreases todo
+    invariant sp == flatten(mapThruKlon((oo - todo), m))
+    invariant done == oo - todo
+    invariant sp == flatten(mapThruKlon((done), m))
+  {
     assert sp == flatten(mapThruKlon((oo - todo), m));
-    assert done == oo - todo == {};
+    var next :| next in todo;
+    assert done == oo - todo;
+    assert done + {next} == oo - (todo - {next});
+    todo := todo - {next};
+    assert done + {next} == oo - todo;
+
+    var sext := m.m[next];
+    assert klonLine(next, sext, m);
+    assert klonIdentity(next, sext, m);
+
+    var sowner;   var fowner;
+
+    if (next == m.o)
+    {
+      assert sext == m.c;
+      sowner := m.clowner;
+      fowner := flatten(m.clowner);
+      assert fowner == flatten(sext.owner);
+    }
+    else if (outside(next, m.o))
+    {
+      assert next == sext; assert next.owner == sext.owner;
+      sowner := next.owner;
+      fowner := flatten(next.owner);
+      assert fowner == flatten(sext.owner);
+    }
+    else
+    {
+      assert strictlyInside(next, m.o);
+      sowner := mapThruKlon(next.owner, m);
+      assert sowner == sext.owner;
+      fowner := recSplatten(next.owner, m);
+      assert fowner == flatten(sext.owner);
+    } //end if elseif else
+
+    assert fowner == flatten(sext.owner);
+    FLATTEN_ONE(sext);
+    assert flatten({sext}) == ({sext} + flatten(sext.owner)) == ({sext} + fowner);
+    MAPPEN_ONE(next,m);
+    assert mapThruKlon({next}, m) == {m.m[next]} == {sext};
+    assert flatten(mapThruKlon({next}, m)) == flatten({sext}) == ({sext} + fowner);
     assert sp == flatten(mapThruKlon((done), m));
+    assert (done+{next}) == (done)+({next});    FLATTEN_SUMS(done,{next},done+{next},m);
+    assert (mapThruKlon((done+{next}), m)) == (mapThruKlon((done), m)) + (mapThruKlon(({next}), m));
+    assert flatten(mapThruKlon((done+{next}), m)) == flatten(mapThruKlon((done), m)) + flatten(mapThruKlon(({next}), m)) == sp + ({sext} + fowner);
+    sp := sp + ({sext} + fowner);
+    done := done + {next};
+    assert done == oo - todo;
+    assert sp == flatten(mapThruKlon((done), m));
+    assert sp == flatten(mapThruKlon((oo - todo), m));
+  }//end while
+  assert sp == flatten(mapThruKlon((oo - todo), m));
+  assert todo == {}; assert done == oo;
+  assert sp == flatten(mapThruKlon(oo, m));
+}
 
-    while (todo > {})
-        decreases todo
-        invariant sp == flatten(mapThruKlon((oo - todo), m))
-        invariant done == oo - todo
-        invariant sp == flatten(mapThruKlon((done), m))
-          {
-            assert sp == flatten(mapThruKlon((oo - todo), m));
-            var next :| next in todo;
-            assert done == oo - todo;
-            assert done + {next} == oo - (todo - {next});
-            todo := todo - {next};
-            assert done + {next} == oo - todo;
 
-            var sext := m.m[next];
-            assert klonLine(next, sext, m);
-            assert klonIdentity(next, sext, m);
 
-            var sowner;   var fowner;
 
-            if (next == m.o)
-              {
-                assert sext == m.c;
-                sowner := m.clowner;
-                fowner := flatten(m.clowner);
-                assert fowner == flatten(sext.owner);
-              }
-            else if (outside(next, m.o))
-              {
-                assert next == sext; assert next.owner == sext.owner;
-                sowner := next.owner;
-                fowner := flatten(next.owner);
-                assert fowner == flatten(sext.owner);
-              }
-            else
-              {
-                assert strictlyInside(next, m.o);
-                sowner := mapThruKlon(next.owner, m);
-                assert sowner == sext.owner;
-                fowner := recSplatten(next.owner, m);
-                assert fowner == flatten(sext.owner);
-              } //end if elseif else
 
-            assert fowner == flatten(sext.owner);
-            FLATTEN_ONE(sext);
-            assert flatten({sext}) == ({sext} + flatten(sext.owner)) == ({sext} + fowner);
-            MAPPEN_ONE(next,m);
-            assert mapThruKlon({next}, m) == {m.m[next]} == {sext};
-            assert flatten(mapThruKlon({next}, m)) == flatten({sext}) == ({sext} + fowner);
-            assert sp == flatten(mapThruKlon((done), m));
-            assert (done+{next}) == (done)+({next});    FLATTEN_SUMS(done,{next},done+{next},m);
-            assert (mapThruKlon((done+{next}), m)) == (mapThruKlon((done), m)) + (mapThruKlon(({next}), m));
-            assert flatten(mapThruKlon((done+{next}), m)) == flatten(mapThruKlon((done), m)) + flatten(mapThruKlon(({next}), m)) == sp + ({sext} + fowner);
-            sp := sp + ({sext} + fowner);
-            done := done + {next};
-            assert done == oo - todo;
-            assert sp == flatten(mapThruKlon((done), m));
-            assert sp == flatten(mapThruKlon((oo - todo), m));
-          }//end while
-      assert sp == flatten(mapThruKlon((oo - todo), m));
-      assert todo == {}; assert done == oo;
-      assert sp == flatten(mapThruKlon(oo, m));
-  }
+//reminder OWNR is flat
+
+
+
+lemma insideThruKlon(below : Owner, above : Owner, m : Klon) returns (rv : bool)
+  decreases allAMFOs(below)
+  requires AllReady(below)
+  requires AllReady(above)
+  requires klonReady(m)
+  requires klonCalid(m)
+  requires below <= m.m.Keys
+  requires above <= m.m.Keys
+
+  requires flatten(below) >= flatten(above)
+  //    ensures rv
+{
+  var pivot := m.o;
+
+  var belowFlat : OWNR := recSplatten(below, m);
+  var aboveFlat : OWNR := recSplatten(above, m);
+
+
+  var belowInside,belowOutside,belowFringe := splitOWNRSroundPivot(below, pivot);
+  assert (belowInside > {}) ==> (pivot in belowFringe);
+  var belowFringeNoPivot := belowFringe - {pivot};
+
+  var aboveInside,aboveOutside,aboveFringe := splitOWNRSroundPivot(above, pivot);
+  assert (aboveInside > {}) ==> (pivot in aboveFringe);
+  var aboveFringeNoPivot := aboveFringe - {pivot};
+
+
+
+  rv := (belowFlat >= aboveFlat);
+  assert rv;
+}
